Lazily add inputs in resetAig

Valaig/Aig/Projections.lean
@@ -10,54 +10,10 @@ variable {aig : Aig} {wf : aig.WellFormed}
 namespace resetAig
 
 @[always_inline]
-private def initLeaves (aig : Aig) : Aig :=
-  aig.inputs.fold addInput' .empty
-
-@[simp, grind .]
-theorem Comb_initLeaves :
-    (initLeaves aig).Comb := by
-  simp only [initLeaves, ←Std.Iter.foldl_toList]
-  apply List.foldlRecOn <;> grind
-
-@[simp, grind .]
-theorem WellFormed_initLeaves :
-    (initLeaves aig).WellFormed := by
-  suffices h : ∀ (list : List InputIdx) (state : Aig),
-      state.WellFormed → list.Nodup → (∀ idx ∈ list, ¬idx.validIn state) →
-      (list.foldl addInput' state).WellFormed by
-    simp only [initLeaves, ←Std.Iter.foldl_toList]
-    grind
-  intro list state
-  induction h : list generalizing list state <;> grind
-
-@[simp, grind =]
-theorem numInputs_initLeaves :
-    (initLeaves aig).numInputs = aig.numInputs := by
-  suffices h : ∀ (list : List InputIdx) (state : Aig),
-      list.Nodup → (∀ idx ∈ list, ¬idx.validIn state) →
-      (list.foldl addInput' state).numInputs = state.numInputs + list.length by
-    simp only [initLeaves, ←Std.Iter.foldl_toList]
-    grind [Std.Iter.length_toList_eq_length]
-  intro list state
-  induction h : list generalizing list state <;> grind
-
-@[simp, grind .]
-theorem input_validIn_initLeaves {idx : InputIdx} (valid : idx.validIn aig) :
-    idx.validIn (initLeaves aig) := by
-  suffices h : ∀ (tail : List InputIdx) (state : Aig),
-      (∀ idx ∉ tail, idx.validIn aig → idx.validIn state) →
-      idx.validIn (tail.foldl addInput' state) by
-    simp only [initLeaves, ←Std.Iter.foldl_toList]
-    grind
-  intro list state
-  induction h : list generalizing list state <;> grind
-
-@[always_inline]
 def step (aig : Aig) (state : Aig) (map : Array Lit) (var : Var)
     (valid : var.validIn aig := by grind)
     (wf : aig.WellFormed := by grind)
-    (inputsValid : {idx : InputIdx} → idx.validIn aig → idx.validIn state := by grind)
-    (valid : ∀ {lit},  lit ∈ map → lit.validIn state := by grind)
+    (valid : ∀ lit ∈ map, lit.validIn state := by grind)
     (size : var.idx = map.size := by grind) :
     Aig × Array Lit :=
   let mapLit (lit : Lit) (h : lit.var < var := by grind) : Lit.In state :=
@@ -66,7 +22,8 @@ def step (aig : Aig) (state : Aig) (map : Array Lit) (var : Var)
   let (eq:=_) (state, lit) : Aig × Lit :=
     match _ : aig[var] with
     | .false         => (state, .false)
-    | .input idx     => (state, idx.getLit state)
+    | .input idx     => let state := state.addInput' idx
+                        (state, idx.getLit state)
     | .latch idx     => (state, mapLit (idx.getReset aig))
     | .and rhs0 rhs1 => state.addAnd (mapLit rhs0) (mapLit rhs1)
 
@@ -76,9 +33,15 @@ variable {state : Aig} {map : Array Lit} {var : Var}
 variable {valid : var.validIn aig}
 variable {wf : aig.WellFormed}
 variable {swf : state.WellFormed}
-variable {inputsValid : {idx : InputIdx} → idx.validIn aig → idx.validIn state}
-variable {valid : ∀ {lit},  lit ∈ map → lit.validIn state}
+variable {valid : ∀ lit ∈ map, lit.validIn state}
 variable {size : var.idx = map.size}
+variable {idxInvalid : ∀ {idx}, aig[var] = .input idx → ¬idx.validIn state}
+
+@[simp, grind .]
+theorem Comb_step (comb : state.Comb) :
+    (step aig state map var).fst.Comb := by
+  unfold step
+  grind
 
 @[simp, grind =]
 theorem size_step :
@@ -87,23 +50,39 @@ theorem size_step :
   grind
 
 @[simp, grind .]
-theorem inputsValid_step {idx : InputIdx} (h : idx.validIn aig) :
+theorem input_validIn_step {idx : InputIdx} (valid : idx.validIn aig)
+    (h : (idx.getVar aig < var ∧ idx.validIn state) ∨ idx.getVar aig = var) :
     idx.validIn (step aig state map var).fst := by
   unfold step
   grind
 
-include swf in
+@[simp, grind .]
+theorem inputs_not_validIn_step {idx : InputIdx} (valid : idx.validIn aig) (invalid : ¬idx.validIn state)
+    (gt : idx.getVar aig > var) :
+    ¬idx.validIn (step aig state map var).fst := by
+  unfold step
+  grind
+
+@[simp, grind .]
+theorem inputsInvalid_step {idx : InputIdx} (h : idx.validIn aig)
+    (hs : (idx.getVar aig < var ∧ idx.validIn state) ∨ idx.getVar aig = var) :
+    idx.validIn (step aig state map var).fst := by
+  unfold step
+  grind
+
+include idxInvalid swf in
 @[simp, grind .]
 theorem WellFormed_step :
     (step aig state map var).fst.WellFormed := by
   unfold step
   grind
 
-include swf in
+include idxInvalid in
 @[simp, grind .]
-theorem valid_step {lit} (h : lit ∈ (step aig state map var).snd) :
+theorem valid_step {lit : Lit}
+   (h : lit ∈ (step aig state map var).snd) :
     lit.validIn (step aig state map var).fst := by
-  simp_all [step]
+  simp_all only [step]
   grind
 
 end resetAig
@@ -114,12 +93,13 @@ latch its reset value. This results in a combinational Aig with the same number 
 and a map to map from literals in the old Aig to the new one.
 -/
 def resetAig (aig : Aig) (wf : aig.WellFormed := by grind) : Aig × (Lit.In aig -> Lit) :=
-  go aig.iter (resetAig.initLeaves aig) (.emptyWithCapacity aig.size)
+  go aig.iter .empty (.emptyWithCapacity aig.size)
 where
   go it state (map : Array Lit)
       (wf : state.WellFormed := by grind)
-      (inputsValid : {idx : InputIdx} → idx.validIn aig → idx.validIn state := by grind)
-      (valid : ∀ {lit},  lit ∈ map → lit.validIn state := by grind)
+      (valid : ∀ lit ∈ map, lit.validIn state := by grind)
+      (inputsInvalid : ∀ {var : Var} {idx h},
+        aig[var]'h = .input idx -> var ≥ aig.iterVal it → ¬idx.validIn state := by grind)
       (size : (aig.iterVal it).idx = map.size := by grind) :=
     match it.step with
     | .done _ =>
@@ -129,66 +109,39 @@ where
       go it' res.fst res.snd
   termination_by it.finitelyManySteps
 
-namespace resetAig
-variable {it : Std.Iter Var} {state : Aig} {map : Array Lit}
-variable {swf : state.WellFormed}
-variable {size : (aig.iterVal it).idx = map.size}
-
-def go.induction
-    (motive : (Aig × (Lit.In aig -> Lit)) -> Prop)
-    (init : motive (state, (go aig wf it state map).snd))
-    (ind :
-      (it : Std.Iter Var) -> (state : Aig) -> (map : Array Lit) ->
-      (swf : state.WellFormed) ->
-      (inputsValid : {idx : InputIdx} → idx.validIn aig → idx.validIn state) ->
-      (valid : ∀ {lit},  lit ∈ map → lit.validIn state) ->
-      (valid' : (aig.iterVal it).validIn aig) ->
-      (size : (aig.iterVal it).idx = map.size) ->
-      (h : motive (state, (go aig wf it state map).snd)) ->
-      motive ((step aig state map <| aig.iterVal it).fst, (go aig wf it state map).snd)) :
-    let res := go aig wf it state map swf inputsValid valid size
-    motive res := by
-  fun_induction go
-  · grind only
-  next ih =>
-    apply ih
-    clear ih
-    grind [go]
-
-def induction
-    (motive : (Aig × (Lit.In aig -> Lit)) -> Prop)
-    (init : motive (initLeaves aig, (go aig wf aig.iter (initLeaves aig) (.emptyWithCapacity aig.size)).snd))
-    (ind :
-      (it : Std.Iter Var) -> (state : Aig) -> (map : Array Lit) ->
-      (swf : state.WellFormed) ->
-      (inputsValid : {idx : InputIdx} → idx.validIn aig → idx.validIn state) ->
-      (valid : ∀ {lit},  lit ∈ map → lit.validIn state) ->
-      (valid' : (aig.iterVal it).validIn aig) ->
-      (size : (aig.iterVal it).idx = map.size) ->
-      (h : motive (state, (go aig wf it state map).snd)) ->
-      motive ((step aig state map <| aig.iterVal it).fst, (go aig wf it state map).snd)) :
-    motive aig.resetAig := by
-  apply go.induction motive <;> grind
-
-end resetAig
-
 @[simp, grind .]
 theorem Comb_resetAig :
     aig.resetAig.fst.Comb := by
-  apply resetAig.induction (·.fst.Comb)
-  <;> (try unfold resetAig.step) <;> grind
+  grind [resetAig, @Comb_go]
+where
+  Comb_go {it state map swf inputsValid valid size} (comb : state.Comb) :
+      (resetAig.go aig wf it state map swf inputsValid valid size).fst.Comb := by
+    fun_induction resetAig.go <;> grind
 
 @[simp, grind .]
 theorem WellFormed_resetAig :
     aig.resetAig.fst.WellFormed := by
-  apply resetAig.induction (·.fst.WellFormed)
-  <;> (try unfold resetAig.step) <;> grind
+  grind [resetAig, @WellFormed_go]
+where
+  WellFormed_go {it state map swf inputsValid valid size} :
+      (resetAig.go aig wf it state map swf inputsValid valid size).fst.WellFormed := by
+    fun_induction resetAig.go <;> grind
+
+@[simp, grind =]
+theorem input_validIn_resetAig {idx : InputIdx} :
+    idx.validIn aig.resetAig.fst ↔ idx.validIn aig := by
+  grind [resetAig, @input_validIn_go]
+where
+  input_validIn_go {it state map swf inputsValid valid size} :
+      let res := resetAig.go aig wf it state map swf inputsValid valid size
+      idx.validIn res.fst ↔
+      idx.validIn state ∨ ∃ h, idx.getVar aig h ≥ (aig.iterVal it) := by
+    fun_induction resetAig.go <;> grind [resetAig.step]
 
 @[simp, grind =]
 theorem numInputs_resetAig :
     aig.resetAig.fst.numInputs = aig.numInputs := by
-  apply resetAig.induction (·.fst.numInputs = aig.numInputs)
-  <;> (try unfold resetAig.step) <;> grind
+  grind [numInputs_eq_of_validIn_eq]
 
 @[simp, grind .]
 theorem resetAig_validIn {lit : Lit.In aig} :
@@ -214,8 +167,9 @@ theorem denote_mapTo (lit : Lit) {lt : lit.var.idx < map.size} :
 
 include denote in
 @[local grind =]
-theorem denote_step {var var' inputsValid valid valid' size} :
-    let res := resetAig.step aig state map var' valid wf inputsValid valid' size
+theorem denote_step {var var' inputsValid valid size}
+    {idxInvalid : ∀ {idx}, aig[var'] = .input idx → ¬idx.validIn state} :
+    let res := resetAig.step aig state map var' valid wf inputsValid size
     (lt : var.idx < res.snd.size) →
       res.fst.denote res.snd[var.idx] 0 assign = aig.denoteVar var 0 assign := by
   intro res h
@@ -234,7 +188,10 @@ theorem denote_go (lit : Lit.In aig) {it inputsValid valid size wf'} :
     res.fst.denote (res.snd lit) 0 assign wf' = aig.denote lit 0 assign := by
   fun_induction resetAig.go
   · grind only [denote_mapTo]
-  · grind only [denote_step]
+  next ih =>
+    apply ih
+    intros
+    apply denote_step <;> grind
 
 end denote_resetAig
 
